updates

intermediate/Veritas.Intermediate.Store.fst
@@ -1187,6 +1187,36 @@ let store_contains_inuse_slot_keys #vcfg (st: ismap_vstore vcfg) (s: inuse_slot_
   : Lemma (ensures (store_contains_key st (stored_key st s))) =
   seq_contains_key st s
 
+let lemma_ismap_madd_to_store1 (#vcfg:_) (st:ismap_vstore vcfg)
+  (s:empty_slot_id st)
+  (k:key) (v:value_type_of k)
+  (s':merkle_slot_id st)
+  (d:bin_tree_dir {points_to_none st s' d})
+  : Lemma (requires (not (store_contains_key st k)))
+          (ensures (is_map (madd_to_store st s k v s' d))) =
+  let stn: vstore vcfg = madd_to_store st s k v s' d in
+  let aux (s: inuse_slot_id stn) (s': inuse_slot_id stn{s' <> s})
+    : Lemma (ensures (stored_key stn s <> stored_key stn s'))
+            [SMTPat (stored_key stn s <> stored_key stn s')] = admit()
+  in
+  admit()
+
+let lemma_ismap_madd_to_store2 (#vcfg:_) (st:ismap_vstore vcfg)
+  (s:empty_slot_id st)
+  (k:key) (v:value_type_of k)
+  (s':merkle_slot_id st)
+  (d:bin_tree_dir {points_to_none st s' d})
+  : Lemma (requires (not (store_contains_key st k)))
+          (ensures (is_map (madd_to_store st s k v s' d))) =
+  let stn:vstore vcfg = madd_to_store st s k v s' d in
+  let aux (s: inuse_slot_id stn) (s': inuse_slot_id stn{s' <> s})
+    : Lemma (ensures (stored_key stn s <> stored_key stn s')) = admit()
+  in
+  forall_intro_2 aux;
+  // assert fails
+  //assert(is_map stn);
+  admit()
+
 let lemma_ismap_madd_to_store (#vcfg:_) (st:ismap_vstore vcfg)
   (s:empty_slot_id st)
   (k:key) (v:value_type_of k)
@@ -1195,10 +1225,16 @@ let lemma_ismap_madd_to_store (#vcfg:_) (st:ismap_vstore vcfg)
   : Lemma (requires (not (store_contains_key st k)))
           (ensures (is_map (madd_to_store st s k v s' d)))
   =
-  let st1 = madd_to_store st s k v s' d in
+  let st1: vstore vcfg = madd_to_store st s k v s' d in
   let aux (s1: inuse_slot_id st1) (s2: inuse_slot_id st1{s2 <> s1}):
-    Lemma (ensures (stored_key st1 s1 <> stored_key st1 s2)) = admit()
-
+    Lemma (ensures (stored_key st1 s1 <> stored_key st1 s2)) =
+    if stored_key st1 s1 <> stored_key st1 s2 then ()
+    else if s1 = s then
+      store_contains_inuse_slot_keys st s2
+    else if s2 = s then
+      store_contains_inuse_slot_keys st s1
+    else
+      ()
   in
   forall_intro_2 aux;
   assert(forall (s1: inuse_slot_id st1) (s2: inuse_slot_id st1{s2 <> s1}). stored_key st1 s1 <> stored_key st1 s2);
@@ -1215,44 +1251,101 @@ let lemma_ismap_madd_to_store_split
   (d2:bin_tree_dir)
   : Lemma (requires (not (store_contains_key st k)))
           (ensures (is_map (madd_to_store_split st s k v s' d d2)))
-  = admit()
+  =
+  let st1: vstore vcfg = madd_to_store_split st s k v s' d d2 in
+  let aux (s1: inuse_slot_id st1) (s2: inuse_slot_id st1{s2 <> s1}):
+    Lemma (ensures (stored_key st1 s1 <> stored_key st1 s2))
+          [SMTPat (stored_key st1 s1 <> stored_key st1 s2)] =
+    if stored_key st1 s1 <> stored_key st1 s2 then ()
+    else if s1 = s then
+      store_contains_inuse_slot_keys st s2
+    else if s2 = s then
+      store_contains_inuse_slot_keys st s1
+    else
+      ()
+  in
+  admit()
 
 let lemma_ismap_correct (#vcfg:_) (st:ismap_vstore vcfg) (s1 s2: inuse_slot_id st)
   : Lemma (requires (stored_key st s1 = stored_key st s2))
           (ensures (s1 = s2))
-  = admit()
+  =
+  ()
 
 let lemma_empty_store_is_map (#vcfg:_):
-  Lemma (ensures (is_map (empty_store vcfg))) = admit()
+  Lemma (ensures (is_map (empty_store vcfg))) = ()
+
+let rec index_of_found #vcfg (st: Seq.seq (option (vstore_entry vcfg))) (k: key{Some? (find st k)}):
+  Tot (i: seq_index st{Some? (Seq.index st i) /\
+                       VStoreE?.k (Some?.v (Seq.index st i)) = k /\
+                       Spec.stored_value (find st) k = VStoreE?.v (Some?.v (Seq.index st i)) /\
+                       Spec.add_method_of (find st) k = VStoreE?.am (Some?.v (Seq.index st i))})
+  (decreases (Seq.length st)) =
+  match Seq.head st with
+  | None -> 1 + index_of_found (Seq.tail st) k
+  | Some (VStoreE k1 v1 am1 _ _ _) ->
+    if k1 = k then 0
+    else 1 + index_of_found (Seq.tail st) k
 
 let lemma_empty_contains_nokey (#vcfg:_) (k:key):
   Lemma (ensures (let st = empty_store vcfg in
-                  not (store_contains_key st k))) = admit()
+                  not (store_contains_key st k))) =
+  let st = empty_store vcfg in
+  if store_contains_key st k then (
+    let i = index_of_found st k in
+    ()
+  )
+  else ()
 
 let lemma_madd_root_to_store_is_map
       (#vcfg:_)
       (st:ismap_vstore vcfg{not (store_contains_key st Root)})
       (s:empty_slot_id st)
       (v:value_type_of Root)
-  : Lemma (ensures (is_map (madd_to_store_root st s v))) = admit()
+  : Lemma (ensures (is_map (madd_to_store_root st s v))) =
+  let st1: vstore vcfg = madd_to_store_root st s v in
+  let aux (s1: inuse_slot_id st1) (s2: inuse_slot_id st1{s2 <> s1}):
+    Lemma (ensures (stored_key st1 s1 <> stored_key st1 s2))
+          [SMTPat (stored_key st1 s1 <> stored_key st1 s2)] =
+    if stored_key st1 s1 <> stored_key st1 s2 then ()
+    else if s1 = s then
+      store_contains_inuse_slot_keys st s2
+    else if s2 = s then
+      store_contains_inuse_slot_keys st s1
+    else
+      ()
+  in
+  admit()
 
 let lemma_as_map_empty (vcfg:_)
   : Lemma (ensures (let st = empty_store vcfg in
-                     forall (k:key). as_map st k = None)) = admit()
+                     forall (k:key). as_map st k = None)) =
+  let st = empty_store vcfg in
+  let aux k: Lemma (ensures (as_map st k = None)) [SMTPat (as_map st k)] =
+    lemma_empty_contains_nokey #vcfg k;
+    ()
+  in
+  ()
 
 let lemma_as_map_slot_key_equiv (#vcfg:_) (st:ismap_vstore vcfg) (s:inuse_slot_id _)
   : Lemma (ensures (let k = stored_key st s in
                     let stk = as_map st in
                     Spec.store_contains stk k /\
                     stored_value st s = Spec.stored_value stk k /\
-                    add_method_of st s = Spec.add_method_of stk k)) = admit()
+                    add_method_of st s = Spec.add_method_of stk k)) =
+  store_contains_inuse_slot_keys st s;
+  let k = stored_key st s in
+  let stk = as_map st in
+  assert(Spec.store_contains stk k);
+  let _ = index_of_found st k in
+  ()
 
 let slot_of_key (#vcfg:_) (st:ismap_vstore vcfg) (k: key{let stk = as_map st in
                                                                   Spec.store_contains stk k})
   : Tot (s: inuse_slot_id st {let stk = as_map st in
                               k = stored_key st s /\
                               stored_value st s = Spec.stored_value stk k /\
-                              add_method_of st s = Spec.add_method_of stk k}) = admit()
+                              add_method_of st s = Spec.add_method_of stk k}) = index_of_found st k
 
 let lemma_not_contains_after_mevict
   (#vcfg: verifier_config)
@@ -1264,7 +1357,19 @@ let lemma_not_contains_after_mevict
   Lemma (ensures (let st' = mevict_from_store st s s' d in
                   let k = stored_key st s in
                   is_map st' /\
-                  not (store_contains_key st' k))) = admit()
+                  not (store_contains_key st' k))) =
+  let st1 = mevict_from_store st s s' d  in
+  let k = stored_key st s in
+  let aux (s1: inuse_slot_id st1) (s2: inuse_slot_id st1{s2 <> s1}):
+    Lemma (ensures (stored_key st1 s1 <> stored_key st1 s2))
+          [SMTPat (stored_key st1 s1 <> stored_key st1 s2)] =
+    assert(s1 <> s /\ s2 <> s);
+    if stored_key st1 s1 <> stored_key st1 s2 then ()
+    else (
+      admit()
+    )
+  in
+  admit()
 
 let lemma_not_contains_after_bevict
   (#vcfg: verifier_config)
@@ -1274,514 +1379,3 @@ let lemma_not_contains_after_bevict
                     let k = stored_key st s in
                     is_map st' /\
                     not (store_contains_key st' k))) = admit()
-
-
-(*
-(* update the data value of a data key *)
-let update_data_value
-  (st:vstore)
-  (s:data_slot_id st)
-  (v:value{DVal? v})
-  : Tot (st':vstore {Seq.length st = Seq.length st' /\
-                     inuse_slot st' s /\
-                     stored_value st' s = v}) =
-  assert(not (desc_in_store st s Left));
-  assert(not (desc_in_store st s Right));
-  let Some (VStoreE k _ am _ _) = get_slot st s in
-  let st' = update_slot st s (VStoreE k v am None None) in
-  assert(Seq.length st = Seq.length st');
-  assert(inuse_slot st' s);
-  assert(stored_value st' s = v);
-
-  let aux1 (s0:slot_id st'):
-    Lemma (ensures (inuse_slot st' s0 = inuse_slot st s0 /\
-                    (inuse_slot st' s0 ==>
-                     stored_key st' s0 = stored_key st s0))) = ()
-  in
-
-  let aux (s0:slot_id st'):
-    Lemma (ensures (store_inv_slot st' s0))
-          [SMTPat (store_inv_slot st' s0)] =
-    if s0 = s then ()
-    else (
-      assert(Seq.index st s0 = Seq.index st' s0);
-      if empty_slot st s0 then ()
-      else if is_data_key (stored_key st s0) then ()
-      else
-        admit()
-    )
-    in
-  assert(store_inv_local st');
-  st'
-
-
-let lemma_lookup_key_returns_k (st:vstore) (k:key)
-  : Lemma (requires (store_contains_key st k))
-          (ensures (VStoreE?.k (Some?.v (lookup_key st k)) = k))
-  = lemma_filter_correct1 (has_key k) st 0
-
-let lemma_lookup_key_returns_None (st:vstore) (k:key)
-  : Lemma (requires (lookup_key st k = None))
-          (ensures (forall i. not (has_key k (Seq.index st i))))
-  = if Seq.length (filter (has_key k) st) = 0
-    then lemma_filter_all_not (has_key k) st
-    else lemma_filter_correct1 (has_key k) st 0
-
-let lemma_store_contains_key (st:vstore) (k:key)
-  : Lemma (requires (exists s. stored_key st s = k))
-          (ensures (store_contains_key st k))
-  = lemma_filter_exists (has_key k) st;
-    lemma_filter_correct1 (has_key k) st 0
-
-let lemma_has_key (st:vstore) (s:slot_id) (k:key)
-  : Lemma (requires (has_key k (get_slot st s)))
-          (ensures (store_contains st s /\ stored_key st s = k))
-  = ()
-
-let lemma_store_contains_key_inv (st:vstore) (k:key)
-  : Lemma (requires (store_contains_key st k))
-          (ensures (exists s. stored_key st s = k))
-  = let s' = filter (has_key k) st in
-    if Seq.length s' > 0
-    then
-      let i = filter_index_map (has_key k) st 0 in
-      lemma_has_key st i k
-
-let stored_value_by_key (st:vstore) (k:key{store_contains_key st k})
-  : value_type_of k
-  = lemma_lookup_key_returns_k st k;
-    VStoreE?.v (Some?.v (lookup_key st k))
-
-let add_method_of_by_key (st:vstore) (k:key{store_contains_key st k})
-  : add_method
-  = VStoreE?.am (Some?.v (lookup_key st k))
-
-(* Two cases where it's safe to add an entry (e) to the store (st) at slot s:
-   * e.k is not in st and s is empty
-   * e.k is already at s *)
-let compatible_entry (st:vstore) (s:st_index st) (e:vstore_entry)
-  = (not (store_contains st s) /\ not (store_contains_key st e.k)) \/
-    (store_contains st s /\ stored_key st s = e.k)
-
-let lemma_update_slot_compatible_entry_is_map
-      (st:vstore{is_map st})
-      (s:st_index st)
-      (e:vstore_entry{compatible_entry st s e})
-  : Lemma (is_map (update_slot st s e))
-          [SMTPat (is_map (update_slot st s e))]
-  = let st_upd = update_slot st s e in
-    let aux (s0:slot_id{store_contains st_upd s0})
-            (s0':slot_id{store_contains st_upd s0' /\ s0' <> s0})
-          : Lemma (stored_key st_upd s0 <> stored_key st_upd s0')
-                  [SMTPat (Seq.index st_upd s0); SMTPat (Seq.index st_upd s0')]
-          = if s0 = s
-            then assert (stored_key st s0' <> e.k)
-            else if s0' = s
-            then assert (stored_key st s0 <> e.k) in
-    assert (is_map st_upd)
-
-let lemma_add_to_store_is_map1
-      (st:vstore)
-      (s:st_index st{not (store_contains st s)})
-      (k:key{not (store_contains_key st k)})
-      (v:value_type_of k)
-      (am:add_method)
-  : Lemma (requires (is_map st))
-          (ensures (is_map (add_to_store st s k v am)))
-  = () // proved by lemma_update_compatible_entry_is_map
-
-let lemma_add_to_store_is_map2
-      (st:vstore)
-      (s:st_index st{not (store_contains st s)})
-      (k:key{store_contains_key st k})
-      (v:value_type_of k)
-      (am:add_method)
-  : Lemma (ensures (~ (is_map (add_to_store st s k v am))))
-  = let st_upd = add_to_store st s k v am in
-    assert (stored_key st_upd s = k);
-    lemma_store_contains_key_inv st k;
-    Classical.exists_elim
-      (exists (s':slot_id{store_contains st_upd s' /\ s' <> s}).
-      stored_key st_upd s' = stored_key st_upd s)
-      (Squash.get_proof (exists s. stored_key st s = k))
-      (fun s' -> assert (stored_key st_upd s' = k));
-    // we have shown two different slots with the same key, so the invariant is violated
-    ()
-
-let lemma_lookup_key_update_value
-      (st:vstore)
-      (s:slot_id{store_contains st s})
-      (v:value_type_of (stored_key st s))
-      (k:key)
-  : Lemma (let res = lookup_key st k in
-           let res' = lookup_key (update_value st s v) k in
-           (None? res /\ None? res') \/
-           (Some? res /\ Some? res' /\ VStoreE?.am (Some?.v res) = VStoreE?.am (Some?.v res')))
-  = let stf = filter (has_key k) st in
-    let Some (VStoreE ks _ am l r) = Seq.index st s in
-    assert (Seq.length stf = Seq.length (filter (has_key k) (update_value st s v)));
-    if Seq.length stf > 0
-    then (
-      if filter_index_map (has_key k) st 0 = s
-      then lemma_filter_update_index_eq (has_key k) st s (Some (VStoreE ks v am l r))
-      else lemma_filter_update_index_neq (has_key k) st s (Some (VStoreE ks v am l r)) 0
-    )
-
-let lemma_update_value_preserves_keys
-      (st:vstore)
-      (s:slot_id{store_contains st s})
-      (v:value_type_of (stored_key st s))
-      (k:key)
-  : Lemma (store_contains_key st k = store_contains_key (update_value st s v) k)
-  = lemma_lookup_key_update_value st s v k
-
-let lemma_update_value_preserves_key_with_MAdd
-  (st:vstore)
-  (s:slot_id{store_contains st s})
-  (v:value_type_of (stored_key st s))
-  (k:key)
-  : Lemma (ensures store_contains_key_with_MAdd st k =
-                     store_contains_key_with_MAdd (update_value st s v) k)
-  = lemma_lookup_key_update_value st s v k
-
-let lemma_add_different_key_to_store_preserves_keys_with_MAdd
-  (st:vstore)
-  (s:st_index st{not (store_contains st s)})
-  (k:key)
-  (v:value_type_of k)
-  (k0:key)
-  : Lemma (requires k <> k0)
-          (ensures store_contains_key_with_MAdd st k0 =
-                     store_contains_key_with_MAdd (add_to_store st s k v Spec.MAdd) k0)
-  = let stf = filter (has_key k0) st in
-    if Seq.length stf > 0
-    then (
-      assert (filter_index_map (has_key k0) st 0 <> s);
-      lemma_filter_update_index_neq (has_key k0) st s (Some (VStoreE k v Spec.MAdd false false)) 0
-    )
-
-let lemma_add_to_store_BAdd_preserves_key_with_MAdd
-  (st:vstore)
-  (s:st_index st{not (store_contains st s)})
-  (k:key{not (store_contains_key st k)})
-  (v:value_type_of k)
-  (k0:key)
-  : Lemma (ensures store_contains_key_with_MAdd st k0 =
-                     store_contains_key_with_MAdd (add_to_store st s k v Spec.BAdd) k0)
-  = let stf = filter (has_key k0) st in
-    if Seq.length stf = 0
-    then (
-      let st_upd = add_to_store st s k v Spec.BAdd in
-      if k = k0
-      then (
-        assert (has_key k0 (Seq.index st_upd s));
-        lemma_filter_all_not (has_key k0) st;
-        assert (forall j. j <> s ==> not (has_key k0 (Seq.index st_upd j)));
-        lemma_filter_unique (has_key k0) st_upd s
-      )
-    )
-    else (
-      lemma_filter_correct1 (has_key k0) st 0;
-      assert (k <> k0);
-      assert (filter_index_map (has_key k0) st 0 <> s);
-      lemma_filter_update_index_neq (has_key k0) st s (Some (VStoreE k v Spec.BAdd false false)) 0
-    )
-
-let lemma_add_to_store_MAdd_adds_key_with_MAdd
-  (st:vstore)
-  (s:st_index st{not (store_contains st s)})
-  (k:key{not (store_contains_key st k)})
-  (v:value_type_of k)
-  : Lemma (ensures store_contains_key_with_MAdd (add_to_store st s k v Spec.MAdd) k)
-  = let st_upd = add_to_store st s k v Spec.MAdd in
-    assert (has_key k (Seq.index st_upd s));
-    lemma_lookup_key_returns_None st k;
-    lemma_filter_all_not (has_key k) st;
-    assert (forall j. j <> s ==> not (has_key k (Seq.index st_upd j)));
-    lemma_filter_unique (has_key k) st_upd s
-
-let lemma_lookup_key_update_in_store
-      (st:vstore)
-      (s:slot_id{store_contains st s})
-      (d:bin_tree_dir)
-      (b:bool)
-      (k:key)
-  : Lemma (let res = lookup_key st k in
-           let res' = lookup_key (update_in_store st s d b) k in
-           (None? res /\ None? res') \/
-           (Some? res /\ Some? res' /\ VStoreE?.am (Some?.v res) = VStoreE?.am (Some?.v res')))
-  = let stf = filter (has_key k) st in
-    let Some (VStoreE ks v am l r) = Seq.index st s in
-    let newelem = match d with
-                  | Left -> Some (VStoreE ks v am b r)
-                  | Right -> Some (VStoreE ks v am l b) in
-    assert (Seq.length stf = Seq.length (filter (has_key k) (update_in_store st s d b)));
-    if Seq.length stf > 0
-    then (
-      (** TODO: For some reason this started failing with the updated vevictb/vevictbm *)
-      (*
-      if filter_index_map (has_key k) st 0 = s
-      then lemma_filter_update_index_eq (has_key k) st s newelem
-      else lemma_filter_update_index_neq (has_key k) st s newelem 0
-      *)
-      admit()
-    )
-
-let lemma_update_in_store_preserves_keys
-  (st:vstore)
-  (s:st_index st{store_contains st s})
-  (d:bin_tree_dir)
-  (b:bool)
-  (k:key)
-  : Lemma (ensures store_contains_key st k = store_contains_key (update_in_store st s d b) k)
-  = lemma_lookup_key_update_in_store st s d b k
-
-let lemma_update_in_store_preserves_key_with_MAdd
-  (st:vstore)
-  (s:st_index st{store_contains st s})
-  (d:bin_tree_dir)
-  (b:bool)
-  (k:key)
-  : Lemma (ensures store_contains_key_with_MAdd st k =
-                     store_contains_key_with_MAdd (update_in_store st s d b) k)
-  = lemma_lookup_key_update_in_store st s d b k
-
-let lemma_evict_from_store_evicts_key
-  (st:vstore)
-  (s:st_index st{store_contains st s})
-  : Lemma (requires is_map st)
-          (ensures not (store_contains_key (evict_from_store st s) (stored_key st s)))
-  = let k = stored_key st s in
-    let st_upd = evict_from_store st s in
-    let res = filter (has_key k) st_upd in
-    lemma_filter_all_not_inv (has_key k) st_upd;
-    assert (Seq.length res = 0)
-
-let lemma_lookup_key_evict_from_store
-      (st:vstore)
-      (s:slot_id{store_contains st s})
-      (k:key{k <> stored_key st s})
-  : Lemma (lookup_key st k = lookup_key (evict_from_store st s) k)
-  = let stf = filter (has_key k) st in
-    if Seq.length stf > 0
-    then (
-      assert (filter_index_map (has_key k) st 0 <> s);
-      lemma_filter_update_index_neq (has_key k) st s None 0
-    )
-
-let lemma_evict_from_store_preserves_key_with_MAdd
-  (st:vstore)
-  (s:st_index st{store_contains st s})
-  (k:key)
-  : Lemma (requires (k <> stored_key st s))
-          (ensures (store_contains_key_with_MAdd st k = store_contains_key_with_MAdd (evict_from_store st s) k))
-  = lemma_lookup_key_evict_from_store st s k
-
-let lemma_get_slot_lookup_key (st:vstore{is_map st}) (s:slot_id) (k:key)
-  : Lemma (requires (store_contains st s /\ stored_key st s = k))
-          (ensures (get_slot st s = lookup_key st k))
-  = let s' = filter (has_key k) st in
-    lemma_filter_unique (has_key k) st s
-
-let lemma_evict_from_store_BAdd_preserves_key_with_MAdd
-  (st:vstore{is_map st})
-  (s:slot_id{store_contains st s})
-  (k:key)
-  : Lemma (requires (add_method_of st s = Spec.BAdd))
-          (ensures (store_contains_key_with_MAdd st k =
-                      store_contains_key_with_MAdd (evict_from_store st s) k))
-  = if k = stored_key st s
-    then lemma_get_slot_lookup_key st s k
-    else lemma_lookup_key_evict_from_store st s k
-
-let lemma_slot_key_equiv_update_value
-      (st:vstore)
-      (s:slot_id)
-      (s':slot_id{store_contains st s'})
-      (k:key)
-      (v:value_type_of (stored_key st s'))
-  : Lemma (requires (slot_key_equiv st s k /\ s <> s'))
-          (ensures (slot_key_equiv (update_value st s' v) s k))
-  = ()
-
-
-let rec lemma_as_map_empty (n:nat)
-  : Lemma (ensures (let st = empty_store n in
-                     forall (k:key). as_map st k = None))
-          (decreases n)
-  = if n <> 0
-    then (
-      lemma_prefix_create n (None #vstore_entry) (n-1);
-      lemma_as_map_empty (n-1)
-    )
-
-let lemma_is_map_prefix (l:vstore) (i:seq_index l)
-  : Lemma (requires (is_map l))
-          (ensures (is_map (prefix l i)))
-          [SMTPat (is_map (prefix l i))]
-  = ()
-
-let rec lemma_as_map_slot_key_equiv_aux
-      (l:vstore)
-      (s:slot_id)
-      (k:key)
-      (v:value_type_of k)
-      (am:add_method)
-      (lb rb:bool)
-  : Lemma (requires (s < Seq.length l /\
-                     Seq.index l s = Some (VStoreE k v am lb rb) /\
-                     is_map l))
-          (ensures (Spec.store_contains (as_map_aux l) k /\
-                    Spec.stored_value (as_map_aux l) k = v /\
-                    Spec.add_method_of (as_map_aux l) k = am))
-          (decreases (Seq.length l))
-  = let n = Seq.length l in
-    if n <> 0
-    then
-      let l' = prefix l (n - 1) in
-      match Seq.index l (n - 1) with
-      | None -> lemma_as_map_slot_key_equiv_aux l' s k v am lb rb
-      | Some (VStoreE k2 v2 am2 _ _) ->
-          if s < n - 1
-          then lemma_as_map_slot_key_equiv_aux l' s k v am lb rb
-
-let lemma_as_map_slot_key_equiv (st:vstore{is_map st}) (s:slot_id) (k:key)
-  : Lemma (requires (slot_key_equiv st s k))
-          (ensures (Spec.store_contains (as_map st) k /\
-                    stored_value st s = Spec.stored_value (as_map st) k /\
-                    add_method_of st s = Spec.add_method_of (as_map st) k))
-  = let Some (VStoreE k v a l r) = get_slot st s in
-    lemma_as_map_slot_key_equiv_aux st s k v a l r
-
-let rec lemma_as_map_aux_does_not_contain_key
-      (l:vstore)
-      (k:key)
-  : Lemma (requires (forall i. not (has_key k (Seq.index l i))))
-          (ensures (not (Spec.store_contains (as_map_aux l) k)))
-          (decreases (Seq.length l))
-  = let n = Seq.length l in
-    if n <> 0
-    then
-      let l' = prefix l (n - 1) in
-      lemma_as_map_aux_does_not_contain_key l' k
-
-let lemma_store_rel_contains_key (st:vstore) (st':Spec.vstore) (k:key)
-  : Lemma (requires (store_rel st st'))
-          (ensures (store_contains_key st k = Spec.store_contains st' k))
-  = if store_contains_key st k
-    then (
-      lemma_store_contains_key_inv st k;
-      Classical.exists_elim
-        (Spec.store_contains (as_map st) k)
-        (Squash.get_proof (exists s. slot_key_equiv st s k))
-        (fun s -> lemma_as_map_slot_key_equiv st s k)
-    )
-    else (
-      lemma_lookup_key_returns_None st k;
-      lemma_as_map_aux_does_not_contain_key st k
-    )
-
-let lemma_store_rel_stored_value (st:vstore) (st':Spec.vstore) (k:key)
-  : Lemma (requires (store_rel st st' /\ store_contains_key st k))
-          (ensures (stored_value_by_key st k = Spec.stored_value st' k))
-  = lemma_store_contains_key_inv st k;
-    Classical.exists_elim
-      (stored_value_by_key st k = Spec.stored_value (as_map st) k)
-      (Squash.get_proof (exists s. slot_key_equiv st s k))
-      (fun s -> lemma_get_slot_lookup_key st s k;
-             lemma_as_map_slot_key_equiv st s k)
-
-let lemma_store_rel_add_method_of (st:vstore) (st':Spec.vstore) (k:key)
-  : Lemma (requires (store_rel st st' /\ store_contains_key st k))
-          (ensures (add_method_of_by_key st k = Spec.add_method_of st' k))
-  = lemma_store_contains_key_inv st k;
-    Classical.exists_elim
-      (add_method_of_by_key st k = Spec.add_method_of (as_map st) k)
-      (Squash.get_proof (exists s. slot_key_equiv st s k))
-      (fun s -> lemma_get_slot_lookup_key st s k;
-             lemma_as_map_slot_key_equiv st s k)
-
-let compatible_entry_prefix (st:vstore) (s:st_index st) (e:vstore_entry) (i:st_index st)
-  : Lemma (requires (compatible_entry st s e /\ s < i))
-          (ensures (compatible_entry (prefix st i) s e))
-          [SMTPat (compatible_entry (prefix st i) s e)]
-  = if not (store_contains st s)
-    then (
-      lemma_lookup_key_returns_None st e.k;
-      lemma_filter_all_not_inv (has_key e.k) (prefix st i)
-    )
-
-#push-options "--fuel 1,1 --ifuel 2,2"
-let rec lemma_as_map_update (st:vstore{is_map st})
-                            (s:st_index st)
-                            (e:vstore_entry{compatible_entry st s e})
-  : Lemma (ensures (let m = as_map st in
-                    let m' = as_map (update_slot st s e) in
-                    m' e.k = Some (Spec.VStore e.v e.am) /\
-                    (forall k. k <> e.k ==> m' k = m k)))
-          (decreases (Seq.length st))
-  = let n = Seq.length st in
-    if n <> 0
-    then
-      let st_upd = update_slot st s e in
-      let st_p = prefix st (n - 1) in
-      let st_upd_p = prefix st_upd (n - 1) in
-      if s < n - 1
-      then (
-        let st_p_upd = update_slot st_p s e in
-        lemma_as_map_update st_p s e;
-        assert (Seq.equal st_p_upd st_upd_p)
-      )
-      else ( // s = n - 1
-        assert (Seq.equal st_p st_upd_p)
-      )
-#pop-options
-
-let lemma_store_rel_update_value (st:vstore) (st':Spec.vstore) (s:slot_id) (k:key) (v:value_type_of k)
-  : Lemma (requires (store_rel st st' /\ slot_key_equiv st s k))
-          (ensures (store_rel (update_value st s v) (Spec.update_store st' k v)))
-  = let Some (VStoreE _ _ am l r) = get_slot st s in
-    lemma_as_map_update st s (VStoreE k v am l r)
-
-let lemma_store_rel_update_in_store (st:vstore) (st':Spec.vstore) (s:slot_id) (d:bin_tree_dir) (b:bool)
-  : Lemma (requires (store_rel st st' /\ store_contains st s))
-          (ensures (store_rel (update_in_store st s d b) st'))
-  = let Some (VStoreE k v am l r) = get_slot st s in
-    assert (slot_key_equiv st s k); // assert needed to trigger pattern
-    let e = match d with
-            | Left -> VStoreE k v am b r
-            | Right -> VStoreE k v am l b in
-    lemma_as_map_update st s e
-
-let lemma_store_rel_add_to_store (st:vstore) (st':Spec.vstore) (s:st_index st) (k:key) (v:value_type_of k) (am:add_method)
-  : Lemma (requires (store_rel st st' /\ not (store_contains st s) /\ not (Spec.store_contains st' k)))
-          (ensures (store_rel (add_to_store st s k v am) (Spec.add_to_store st' k v am)))
-  = lemma_as_map_update st s (VStoreE k v am false false)
-
-let rec lemma_as_map_evict (st:vstore{is_map st}) (s:st_index st) (k:key)
-  : Lemma (requires (slot_key_equiv st s k))
-          (ensures (let m = as_map st in
-                    let m' = as_map (evict_from_store st s) in
-                    m' k = None /\ (forall k'. k' <> k ==> m' k' = m k')))
-          (decreases (Seq.length st))
-  = let n = Seq.length st in
-    if n <> 0
-    then
-      let stupd = evict_from_store st s in
-      let stp = prefix st (n - 1) in
-      let stupdp = prefix stupd (n - 1) in
-      if s < n - 1
-      then (
-        lemma_as_map_evict stp s k;
-        assert (Seq.equal stupdp (evict_from_store stp s))
-      )
-      else (  // s = n - 1
-        assert (Seq.equal stp stupdp);
-        lemma_as_map_aux_does_not_contain_key stp k
-      )
-
-let lemma_store_rel_evict_from_store (st:vstore) (st':Spec.vstore) (s:st_index st) (k:key)
-  : Lemma (requires (store_rel st st' /\ slot_key_equiv st s k))
-          (ensures (store_rel (evict_from_store st s) (Spec.evict_from_store st' k)))
-  = lemma_as_map_evict st s k
-*)
